src/HOL/CVC/SMT_Word.thy
@@ -806,10 +806,7 @@ fun
   (*SMT-LIB3 Syntax. First, we wanted to automatically map SMT-LIB2 syntax to this in preprocessing
     but decided against it in case that there are changes other than syntax*)
   (*TODO: Move into its own parser*)
-   bv_term_parser (SMTLIB.Sym "extract",[ i, j ,t])
-       = SOME (mk_extract_from_terms i j t)
-
-  | bv_term_parser (SMTLIB.Sym "@bbT", xs) = (*old name, now bbterm eventually remove*)
+  bv_term_parser (SMTLIB.Sym "@bbT", xs) = (*old name, now bbterm eventually remove*)
         SOME ((Const ("Reversed_Bit_Lists.of_bl", \<^typ>\<open>HOL.bool list\<close> --> mk_wordT(length xs))) 
         $ ((Const (\<^const_name>\<open>List.rev\<close>, \<^typ>\<open>HOL.bool list\<close> -->  \<^typ>\<open>HOL.bool list\<close>)) $ (HOLogic.mk_list \<^typ>\<open>bool\<close> xs)))
   | bv_term_parser (SMTLIB.Sym "@bbterm", xs) =
@@ -995,23 +992,20 @@ end
       SOME (HOLogic.mk_binop \<^const_name>\<open>Rings.divide\<close> (mk_unary \<^const_name>\<open>unsigned\<close> t1, mk_unary \<^const_name>\<open>unsigned\<close> t2))
  | bv_term_parser (SMTLIB.Sym "bvudiv", [t1,t2]) =
       SOME (HOLogic.mk_binop \<^const_name>\<open>smt_udiv\<close> (t1, t2)) (*TODO: What about the case whre t2 is 0? SMTLIB semantics says it should be mask *)
-  | bv_term_parser (SMTLIB.Sym "bvlshr", [t1, t2]) = 
-    let
-      val T1 = fastype_of t1
-    in
-      SOME (Const (\<^const_name>\<open>semiring_bit_operations_class.drop_bit\<close>, \<^typ>\<open>Nat.nat\<close> --> T1 --> T1) $ (Const ( \<^const_name>\<open>unsigned\<close>, T1 --> \<^typ>\<open>Nat.nat\<close> ) $ t2) $ t1)
-   end
+ 
   | bv_term_parser (SMTLIB.Sym "bvashr", [t1, t2]) = 
     let
       val T1 = fastype_of t1
     in
       SOME (Const (\<^const_name>\<open>signed_drop_bit\<close>, \<^typ>\<open>Nat.nat\<close> --> T1 --> T1) $ (Const ( \<^const_name>\<open>unsigned\<close>, T1 --> \<^typ>\<open>Nat.nat\<close> ) $ t2) $ t1)
    end
-  | bv_term_parser (SMTLIB.S[SMTLIB.Sym "_", SMTLIB.Sym "@bit_of",num], [t1]) = 
+  | bv_term_parser (SMTLIB.S[SMTLIB.Sym "_", SMTLIB.Sym "@bit_of",SMTLIB.Num num], [t1]) = 
     let
-      (*val _ = @{print}("here")*)
+      val T1 = fastype_of t1
+      val t2 = HOLogic.mk_number @{typ nat} num
+
     in
-      SOME (Const (\<^const_name>\<open>True\<close>, \<^typ>\<open>bool\<close>))
+      SOME (Const (\<^const_name>\<open>bit\<close>, T1 --> @{typ nat} --> @{typ bool}) $ t1 $ t2)
    end
  
 
